util.v
@@ -25,3 +25,6 @@ Tactic Notation "SSSSCase" constr(name) := Case_aux SSSSCase name.
 Tactic Notation "SSSSSCase" constr(name) := Case_aux SSSSSCase name.
 Tactic Notation "SSSSSSCase" constr(name) := Case_aux SSSSSSCase name.
 Tactic Notation "SSSSSSSCase" constr(name) := Case_aux SSSSSSSCase name.
+
+Definition subset {X:Type} (s s': set X) : Prop :=
+  forall x, set_In x s -> set_In x s'.
